Fixed imports and interesting_bit, added CDH assumption, started reduction step

ntor/Games.ec
@@ -1,6 +1,9 @@
 (* Intermediate Games *)
-require import AllCore FMap FSet Distr NTOR NTOR_nosid.
-import GAKE_mod HRO_mod_c DH.DDH DH.G DH.GP DH.FD.
+require import AllCore FMap FSet Distr.
+
+require NTOR_nosid.
+clone import NTOR_nosid as NTOR_nosid_c.
+import NTORc GAKE_mod DH.G DH.GP DH.FD.
 
 
 (* Proof:
@@ -450,18 +453,10 @@ print Game3.
 
 (* Step4: Replacing key computation on real side with sampling *)
 module Game4 = Game3 with {
-  var counti : int
-  var handles_c : (int, int) fmap
   var test_ephrev_s : bool option
-  var b_test : pkey option
-  var j_test : int option
 
   proc init_mem [
-    -1 + { counti <- 0; handles_c <- empty; test_ephrev_s <- None; b_test <- None; j_test <- None; }
-  ]
-
-  proc send_msg1 [
-    ^if.^match#None.^if.^r<- + {counti <- counti + 1; handles_c.[counti] <- i;}
+    -1 + { test_ephrev_s <- None; }
   ]
 
   proc send_msg2 [
@@ -497,19 +492,17 @@ module Game4 = Game3 with {
     var p : (pkey * int)
     ^if.^match#Some.^match#Accepted.^if.^if.^k<- ~ {ks <$ dkey; if (x \notin h2m) {h2m.[x] <- ks;} k <- h2m.[x]; 
                                                     p <- pick (get_fresh_partners_c t' s_smap servers); 
-                                                    test_ephrev_s <- Some (get_ir_eph (oget s_smap.[p]));
-                                                    b_test <- Some p.`1; j_test <- Some p.`2;}
+                                                    test_ephrev_s <- Some (get_ir_eph (oget s_smap.[p]));}
     ^if.^match#Some.^match#Accepted.^if.^if?^ks<$ + ^ {ks2 <$ dkey; if (x \notin h2m) {h2m.[x] <- ks2;} k <- h2m.[x];
                                                        p <- pick (get_fresh_partners_c t' s_smap servers); 
-                                                       test_ephrev_s <- Some (get_ir_eph (oget s_smap.[p]));
-                                                       b_test <- Some p.`1; j_test <- Some p.`2;}
+                                                       test_ephrev_s <- Some (get_ir_eph (oget s_smap.[p]));}
 
   ]
 
   proc s_test [
     var ks2 : key
-    ^if.^match#Some.^match#Accepted.^if.^if.^k<- ~ {ks <$ dkey; if (x \notin h2m) {h2m.[x] <- ks;} k <- h2m.[x]; test_ephrev_s <- Some ir'.`1; b_test <- Some b; j_test <- Some j;}
-    ^if.^match#Some.^match#Accepted.^if.^if?^ks<$ + ^ {ks2 <$ dkey; if (x \notin h2m) {h2m.[x] <- ks2;} k <- h2m.[x]; test_ephrev_s <- Some ir'.`1; b_test <- Some b; j_test <- Some j;}
+    ^if.^match#Some.^match#Accepted.^if.^if.^k<- ~ {ks <$ dkey; if (x \notin h2m) {h2m.[x] <- ks;} k <- h2m.[x]; test_ephrev_s <- Some ir'.`1;}
+    ^if.^match#Some.^match#Accepted.^if.^if?^ks<$ + ^ {ks2 <$ dkey; if (x \notin h2m) {h2m.[x] <- ks2;} k <- h2m.[x]; test_ephrev_s <- Some ir'.`1;}
   ]
 }.
 
