ntor/St_CDH.ec
@@ -1,0 +1,107 @@
+require import AllCore Distr List FSet FMap.
+require GAKE DiffieHellman.
+
+clone DiffieHellman as DH.
+import DH.DDH DH.G DH.GP DH.FD.
+
+module type Oracle = {
+  proc ddh(x y z : group) : bool
+  proc gen1() : group
+  proc gen2() : group
+  proc corrupt1(i : int) : exp option
+  proc corrupt2(j : int) : exp option
+}.
+
+module type Oracle_i = {
+  include Oracle
+
+  proc init_mem() : unit
+}.
+
+module St_CDH_O : Oracle_i = {
+  var win : bool
+  var n, m : int
+  var cr1, cr2 : int fset
+  var x_map : (int, exp) fmap
+  var y_map : (int, exp) fmap
+
+  proc init_mem() : unit = {
+    win <- false;
+    n <- 0;
+    m <- 0;
+    cr1 <- fset0;
+    cr2 <- fset0;
+    x_map <- empty;
+    y_map <- empty;
+  }
+
+  proc ddh(x y z : group) : bool = {
+    var r <- false;
+
+    if (exists i, i \in x_map /\ x = g ^ (oget x_map.[i]) /\ z = y ^ (oget x_map.[i]) /\ i \notin cr1) {
+      if (exists j, j \in y_map /\ y = g ^ (oget y_map.[j]) /\ j \notin cr2) {
+         win <- true;
+         r <- true;
+      }
+    } elif (exists j, j \in y_map /\ y = g ^ (oget y_map.[j]) /\ z = x ^ (oget y_map.[j])) {
+         r <- true;
+    }
+
+    return r;
+  }
+
+  proc gen1() : group = {
+    var x_n;
+
+    n <- n + 1;
+    x_n <$ dt;
+    x_map.[n] <- x_n;
+
+    return (g ^ x_n);
+  }
+
+  proc gen2() : group = {
+    var y_m;
+
+    m <- m + 1;
+    y_m <$ dt;
+    y_map.[m] <- y_m;
+
+    return (g ^ y_m);
+  }
+
+  proc corrupt1(i : int) : exp option = {
+    var r <- None;
+
+    if (i \in x_map) {
+      cr1 <- cr1 `|` fset1 i;
+      r <- x_map.[i];
+    }
+
+    return r;
+  }
+
+  proc corrupt2(j : int) : exp option = {
+    var r <- None;
+
+    if (j \in y_map) {
+      cr2 <- cr2 `|` fset1 j;
+      r <- y_map.[j];
+    }
+
+    return r;
+  }
+}.
+
+module type Adversary (O : Oracle) = {
+  proc solve() : unit
+}.
+
+(*
+module St_CDH (A : Adversary) (O : Oracle_i) = {
+  proc main(): bool = {
+    
+    r <@ A.solve(O);
+    return (r = g ^ (x * y));
+  }
+}.*)
